test/tactic.lean
@@ -3,6 +3,7 @@ import temporal_logic
 
 open temporal predicate
 
+section
 variable α : Type
 
 variables Γ p q r : cpred
@@ -41,4 +42,65 @@ example (h : Γ ⊢ ◇(◻(f ! v₀ ≡ q) ⋀ p))
 : Γ ⊢ ◇(◻(f ! v₁ ≡ q) ⋀ p) :=
 begin [temporal]
   rw h₂ at h,
+end
+end
+
+inductive nat.even : ℕ → Prop
+ | zero : nat.even 0
+ | succ_succ (n) : nat.even n → nat.even (nat.succ (nat.succ n))
+
+section
+open nat
+lemma even_succ_succ (n : ℕ)
+: nat.even (nat.succ $ nat.succ n) ↔ nat.even n :=
+sorry
+end
+abbreviation succ : var ℕ ℕ := ⟨ nat.succ ⟩
+abbreviation even : var ℕ Prop := ⟨ nat.even ⟩
+
+variables Γ : cpred
+
+example (x y : tvar ℕ)
+(h₀ : Γ ⊢ ◻(⊙x ≃ succ!succ!x))
+(h₁ : Γ ⊢ ◻(⊙y ≃ y))
+(h₂ : Γ ⊢ even!x ≡ even!y)
+: Γ ⊢ ◻(even!x ≡ even!y) :=
+begin [temporal]
+  apply induct _ _ _ _,
+-- h₀ : ◻(⊙x ≃ succ ! succ ! x),
+-- h₁ : ◻(⊙y ≃ y),
+-- h₂ : even ! x ≡ even ! y
+-- ⊢ ◻((even ! x ≡ even ! y) ⟶ ⊙(even ! x ≡ even ! y))
+  { clear h₂,
+    henceforth at ⊢ h₀ h₁,
+-- _inst_1 : persistent Γ,
+-- h₁ : ⊙y ≃ y,
+-- h₀ : ⊙x ≃ succ ! succ ! x
+-- ⊢ (even ! x ≡ even ! y) ⟶ ⊙(even ! x ≡ even ! y)
+    intros h₃,
+-- h₁ : ⊙y ≃ y,
+-- h₀ : ⊙x ≃ succ ! succ ! x,
+-- h₃ : even ! x ≡ even ! y
+-- ⊢ ⊙(even ! x ≡ even ! y)
+    explicit'
+-- x x' y y' : ℕ,
+-- h₃ : nat.even x ↔ nat.even y,
+-- h₀ : x' = nat.succ (nat.succ x),
+-- h₁ : y' = y
+-- ⊢ nat.even x' ↔ nat.even y'
+    { have := even_succ_succ x,
+-- x x' y y' : ℕ,
+-- h₃ : nat.even x ↔ nat.even y,
+-- h₀ : x' = nat.succ (nat.succ x),
+-- h₁ : y' = y,
+-- this : nat.even (nat.succ (nat.succ x)) ↔ nat.even x
+-- ⊢ nat.even x' ↔ nat.even y'
+      guard_hyp h₀ := x' = nat.succ (nat.succ x),
+      guard_target (nat.even x' ↔ nat.even y'),
+      cc, } },
+-- h₀ : ◻(⊙x ≃ succ ! succ ! x),
+-- h₁ : ◻(⊙y ≃ y),
+-- h₂ : even ! x ≡ even ! y
+-- ⊢ even ! x ≡ even ! y
+  { assumption },
 end
