src/temporal_logic/refinement/many_to_many.lean
@@ -1,0 +1,518 @@
+import .simulation
+
+universe variables u u₀ u₁ u₂ u₃
+open predicate nat
+
+namespace temporal
+
+namespace many_to_many
+section
+open fairness
+parameters {α : Type u} {β : Type u₀} {γ : Type u₁ }
+parameters {aevt : Type u₂} {cevt : Type u₃}
+parameters {p : pred' (γ×α)} {q : pred' (γ×β)}
+parameters (A : aevt → act (γ×α)) (C : cevt → act (γ×β))
+parameters {cs₀ fs₀ : aevt → pred' (γ×α)} {cs₁ fs₁ : cevt → pred' (γ×β)}
+parameters (J : pred' (γ×α×β))
+parameter ref : aevt → cevt → Prop
+parameter wit : Π a, subtype (ref a) → cpred
+
+open prod
+
+abbreviation ae (i : aevt) : event (γ×α) := ⟨cs₀ i,fs₀ i,A i⟩
+abbreviation ce (i : cevt) : event (γ×β) := ⟨cs₁ i,fs₁ i,C i⟩
+
+abbreviation ae' (i : aevt) : event (γ×α×aevt) :=
+{ p := cs₀ i!⟨prod.map_right fst⟩
+, q := fs₀ i!⟨prod.map_right fst⟩
+, A := λ s s', s.2.2 = i ∧ (A i on prod.map_right fst) s s' }
+abbreviation ce' (i : cevt) : event (γ×β× cevt) :=
+{ p := cs₁ i!⟨prod.map_right fst⟩
+, q := fs₁ i!⟨prod.map_right fst⟩
+, A := λ s s', s.2.2 = i ∧ (C i on prod.map_right fst) s s' }
+
+section specs
+
+parameters p q cs₀ fs₀ cs₁ fs₁
+
+def SPEC₀.saf (v : tvar α) (o : tvar γ) : cpred :=
+p ! ⦃ o,v ⦄ ⋀
+◻(∃∃ i, ⟦ o,v | A i ⟧)
+
+def SPEC₀ (v : tvar α) (o : tvar γ) : cpred :=
+SPEC₀.saf v o ⋀
+∀∀ i, sched (cs₀ i ! ⦃o,v⦄) (fs₀ i ! ⦃o,v⦄) ⟦ o,v | A i ⟧
+
+def SPEC₁ (v : tvar β) (o : tvar γ) : cpred :=
+q ! ⦃ o,v ⦄ ⋀
+◻(∃∃ i, ⟦ o,v | C i ⟧) ⋀
+∀∀ i, sched (cs₁ i ! ⦃o,v⦄) (fs₁ i ! ⦃o,v⦄) ⟦ o,v | C i ⟧
+
+def SPEC₂ (v : tvar β) (o : tvar γ) (s : tvar cevt) : cpred :=
+q ! ⦃ o,v ⦄ ⋀
+◻(∃∃ i, s ≃ ↑i ⋀ ⟦ o,v | C i ⟧) ⋀
+∀∀ i, sched (cs₁ i ! ⦃o,v⦄) (fs₁ i ! ⦃o,v⦄) (s ≃ ↑i ⋀ ⟦ o,v | C i ⟧)
+
+end specs
+
+parameters [inhabited α] [inhabited cevt] [inhabited aevt]
+
+parameter Hc2a : ∀ ce : cevt, ∃ ae : aevt, ref ae ce
+
+parameter SIM₀ : ∀ v o, (o,v) ⊨ q → ∃ w, (o,w) ⊨ p ∧ (o,w,v) ⊨ J
+parameter SIM
+: ∀ w v o v' o' ce,
+  (o,w,v) ⊨ J →
+  C ce (o,v) (o',v') →
+  ∃ ae w', (o',w',v') ⊨ J ∧
+           ref ae ce ∧
+           A ae (o,w) (o',w')
+
+section obligations
+
+parameters (v : tvar β) (o : tvar γ)
+parameters (Γ : cpred)
+
+parameters β γ
+variable Hpo : ∀ (e : aevt) (w : tvar α),
+  many_to_many_po'
+    (subtype (ref e))
+    (SPEC₁ v o ⋀ SPEC₀.saf w o ⋀ ◻(J ! ⦃o,w,v⦄))
+    (wit e)
+    (λ e', ce e') (ae e)
+    ⦃o,v⦄ ⦃o,w⦄
+parameters {β γ}
+
+section conc_sch
+
+parameters (sch_c : tvar cevt)
+
+variable (sch_a : tvar aevt)
+
+section SPEC₂
+variable H : Γ ⊢ SPEC₂ v o sch_c
+
+open prod temporal.prod
+
+def Next_a : act $ γ × aevt × α :=
+λ σ σ',
+∃ e, σ.2.1 = e ∧ (A e on map_right snd) σ σ'
+
+def Next_c : act $ γ × cevt × β :=
+λ σ σ',
+∃ e, σ.2.1 = e ∧ (C e on map_right snd) σ σ'
+
+section J
+def J' : pred' (γ × (aevt × α) × (cevt × β)) :=
+J ! ⟨ prod.map_right $ prod.map prod.snd prod.snd ⟩ ⋀
+⟨ λ ⟨_, a, c⟩, ref a.1 c.1 ⟩
+
+def p' : pred' (γ × aevt × α) :=
+p ! ⟨prod.map_right prod.snd⟩
+
+def q' : pred' (γ × cevt × β) :=
+q ! ⟨prod.map_right prod.snd⟩
+
+end J
+variable w : tvar α
+open function
+
+noncomputable def Wx₀_f : tvar (β → γ → aevt × α) :=
+λ v o, ε w : aevt × _, (o,w.2) ⊨ p ∧ (o,w.2,v) ⊨ J
+
+noncomputable def Wx₀ : tvar (aevt × α) :=
+Wx₀_f v o
+
+noncomputable def Wf_f : tvar (cevt → β → γ → γ → aevt × α → aevt × α) :=
+⟪ℕ, λ ce v' o o' (w : _ × _),
+      ε w' : aevt × α,
+             (o',w'.2,v') ⊨ J ∧
+             ref w'.1 ce ∧
+             A w'.1 (o,w.2) (o',w'.2) ⟫
+
+noncomputable def Wf : tvar (aevt × α → aevt × α) :=
+Wf_f sch_c (⊙v) o (⊙o)
+
+noncomputable def Wtn (w : tvar (aevt × α)) :=
+w ≃ Wx₀ ⋀ ◻(⊙w ≃ Wf w)
+
+lemma Wx₀_def' (σ : ℕ)
+: σ ⊨ Wx₀ =
+  ε w : _ × α, (σ ⊨ o,w.2) ⊨ p ∧ (σ ⊨ o,w.2,σ ⊨ v) ⊨ J :=
+by repeat { unfold_coes <|> simp [Wx₀,Wx₀_f] }
+
+@[simp,predicate]
+lemma Wx₀_def (σ : ℕ) (a b)
+: (a,b) = σ ⊨ Wx₀ ↔
+  a = (ε w : _ × α,    (σ ⊨ o,w.2) ⊨ p ∧ (σ ⊨ o,w.2,σ ⊨ v) ⊨ J).fst ∧
+  b = (ε w : aevt × α, (σ ⊨ o,w.2) ⊨ p ∧ (σ ⊨ o,w.2,σ ⊨ v) ⊨ J).snd :=
+by repeat { unfold_coes <|> simp [Wx₀,Wx₀_f,ext] }
+
+lemma Wf_def' (σ : ℕ) (w)
+: σ ⊨ Wf ⦃sch_a,w⦄ =
+  ε w' : _ × α,
+         (succ σ ⊨ o,w'.2,succ σ ⊨ v) ⊨ J ∧
+               ref w'.1 (σ ⊨ sch_c) ∧
+               A w'.1 (σ ⊨ o,σ ⊨ w) (succ σ ⊨ o,w'.2) :=
+by repeat { unfold_coes <|> simp [Wf,Wf_f] }
+
+@[simp,predicate]
+lemma Wf_def (σ : ℕ) (w) (a b)
+: (a,b) = σ ⊨ Wf ⦃sch_a,w⦄ ↔
+  a = (ε w' : _ × α,
+         (succ σ ⊨ o,w'.2,succ σ ⊨ v) ⊨ J ∧
+               ref w'.1 (σ ⊨ sch_c) ∧
+               A w'.1 (σ ⊨ o,σ ⊨ w) (succ σ ⊨ o,w'.2)).1 ∧
+  b = (ε w' : aevt × α,
+         (succ σ ⊨ o,w'.2,succ σ ⊨ v) ⊨ J ∧
+               ref w'.1 (σ ⊨ sch_c) ∧
+               A w'.1 (σ ⊨ o,σ ⊨ w) (succ σ ⊨ o,w'.2)).2 :=
+by repeat { unfold_coes <|> simp [Wf,Wf_f,ext] }
+
+variable valid_witness
+: Γ ⊢ Wtn ⦃sch_a,w⦄
+
+lemma abstract_sch (e : aevt)
+: Γ ⊢ sch_a ≃ e ⋀ ⟦ o,w | A e ⟧ ≡ sch_a ≃ e ⋀ ⟦ o,sch_a,w | Next_a ⟧ :=
+begin
+  lifted_pred,
+  split ; intro h ; split
+  ; cases h with h₀ h₁ ; try { assumption },
+  { simp [Next_a,on_fun,h₀], auto, },
+  { simp [Next_a,on_fun,h₀] at h₁, auto }
+end
+
+section Simulation_POs
+-- include SIM₀ Hc2a
+-- lemma SIM₀' (v : cevt × β) (o : γ)
+--   (h : (o, v) ⊨ q')
+-- : (∃ (w : aevt × α), (o, w) ⊨ p' ∧ (o, w, v) ⊨ J') :=
+-- begin
+--   simp [q',prod.map_left] at h,
+--   specialize SIM₀ v.2 o h,
+--   specialize Hc2a v.1,
+--   revert SIM₀, intros_mono,
+--   simp [J',p',map], intros,
+--   cases Hc2a,
+--   constructor_matching* [Exists _, _ ∧ _] ;
+--   tauto,
+-- end
+
+-- omit SIM₀
+-- include SIM
+-- lemma SIM' (w : aevt × α) (v : cevt × β) (o : γ) (v' : cevt × β) (o' : γ)
+--   (h₀ : (o, w, v) ⊨ J')
+--   (h₁ : Next_c (o, v) (o', v'))
+-- : (∃ w', Next_a (o,w) (o',w') ∧ (o', w', v') ⊨ J') :=
+-- begin
+--   simp [J',map] at h₀,
+--   simp [Next_c,on_fun] at h₁,
+--   cases h₀,
+--   specialize SIM w.2 v.2 o v'.2 o' v.1 w.1 h₀_right h₀_left h₁,
+--   cases SIM with w' SIM,
+--   cases Hc2a v'.1 with ae',
+--   existsi [(ae',w')],
+--   simp [Next_a, J',on_fun,map,h₀_right],
+--   tauto,
+-- end
+
+-- include H
+-- omit SIM
+-- lemma H'
+-- : Γ ⊢ simulation.SPEC₁ q' Next_c ⦃v,sch_c⦄ o :=
+-- begin [temporal]
+--   simp [SPEC₂,simulation.SPEC₁,q'] at H ⊢,
+--   split, tauto,
+--   casesm* _ ⋀ _,
+--   persistent,
+--   select h : ◻p_exists _,
+--   henceforth at h ⊢,
+--   cases h with e h,
+--   simp only [Next_c] at *,
+--   explicit'
+--   { cc },
+-- end
+
+-- omit H
+abbreviation ref' : tvar (aevt → cevt → Prop) :=
+ref
+
+-- variable Hcorrect_sched : Γ ⊢ ◻(ref' sch_a sch_c)
+
+include SIM₀ SIM H valid_witness
+
+lemma J_inv_in_w
+: Γ ⊢ ◻(J ! ⦃o,w,v⦄) :=
+begin [temporal]
+  simp [Wtn,SPEC₂] at valid_witness H,
+  cases valid_witness with h₀ h₀,
+  casesm* _ ⋀ _,
+  apply induct _ _ _ _,
+  { persistent,
+    select H₀ : ◻p_exists _,
+    henceforth at h₀ H₀ ⊢,
+    explicit'
+    { intro h,
+      cases h₀, subst w',
+      apply_epsilon_spec, simp, tauto, } },
+  { select Hw : _ ≃ temporal.many_to_many.Wx₀,
+    select Hq : q ! _,
+    clear_except Hw SIM₀ Hq,
+    explicit'
+    { cases Hw, subst w, apply_epsilon_spec,
+      simp, tauto, } }
+end
+
+lemma witness_imp_SPEC₀_saf
+  (h : Γ ⊢ Wtn ⦃sch_a,w⦄)
+: Γ ⊢ SPEC₀.saf w o :=
+begin [temporal]
+  have hJ := temporal.many_to_many.J_inv_in_w sch_a H w valid_witness ,
+  clear valid_witness,
+  simp [SPEC₀.saf,SPEC₂,Wtn] at h ⊢ H,
+  casesm* _ ⋀ _,
+  split,
+  { clear SIM,
+    henceforth at hJ,
+    select Hw : _ ≃ temporal.many_to_many.Wx₀,
+    select h' : q ! _,
+    -- rw [← pair.snd_mk sch_a w,h],
+    explicit'
+    { cases Hw, subst w,
+      apply_epsilon_spec,
+      simp, auto, } },
+  { clear SIM₀,
+    select h : ◻(_ ≃ _),
+    select h' : ◻(p_exists _),
+    persistent,
+    henceforth at h h' ⊢ hJ ,
+    explicit'
+    { cases h, subst w',
+      apply_epsilon_spec,
+      simp, auto, } },
+end
+
+omit H
+parameters p q cs₁ fs₁
+include Hpo p
+omit valid_witness
+
+lemma SPEC₂_imp_SPEC₁
+: (SPEC₂ v o sch_c) ⟹ (SPEC₁ v o) :=
+begin [temporal]
+  simp only [SPEC₁,SPEC₂,temporal.many_to_many.SPEC₁,temporal.many_to_many.SPEC₂],
+  monotonicity, apply ctx_p_and_p_imp_p_and',
+  { monotonicity, simp, intros x h₀ h₁,
+    existsi x, exact h₁ },
+  { intros h i h₀ h₁,
+    replace h := h _ h₀ h₁,
+    revert h, monotonicity, simp, }
+end
+
+section
+omit Hpo
+include valid_witness fs₁ cs₁ Γ H
+-- #check w
+-- noncomputable def sch_w : tvar aevt :=
+-- ⟪ ℕ, λ (w w' : α), ε ae, A ae w w' ⟫ w (⊙w)
+
+lemma sch_w_spec
+: Γ ⊢ ◻(ref' (⊙sch_a) sch_c) :=
+begin [temporal]
+  have hJ := temporal.many_to_many.J_inv_in_w _ H _ valid_witness,
+  simp [Wtn,SPEC₂] at valid_witness H,
+  cases valid_witness with Hw Hw,
+  cases H with H H',
+  cases H with H H,
+  persistent,
+  -- have H' := temporal.many_to_many.H',
+  henceforth at Hw ⊢ hJ H,
+  explicit'
+  { cases Hw, subst sch_a', apply_epsilon_spec,
+    simp, apply SIM ; auto, },
+end
+
+end
+
+include H valid_witness
+lemma H_C_imp_A (e : cevt) (e' : aevt)
+  -- (Hsim : ref e' e)
+: Γ ⊢ ◻(sch_c ≃ ↑e ⟶ ⊙sch_a ≃ ↑e' ⟶ ⟦ o,v | C e ⟧ ⟶ ⟦ o,w | A e' ⟧) :=
+begin [temporal]
+  have hJ := temporal.many_to_many.J_inv_in_w sch_a H w valid_witness,
+  simp [Wtn] at valid_witness,
+  cases valid_witness with h₀ h₁,
+  clear_except hJ SIM h₁,
+  persistent,
+  henceforth at *,
+  explicit'
+  { intros, cases h₁, subst w', subst sch_a', substs e',
+    apply_epsilon_spec,
+    simp, subst e,
+    tauto, },
+end
+omit valid_witness H
+/- latest idea: sch_a should be part of concrete state?
+-/
+
+lemma Hpo' (e : aevt)
+: many_to_many_po'
+     (subtype (ref e)) (SPEC₂ v o sch_c ⋀ Wtn ⦃sch_a,w⦄ ⋀ ◻(J ! ⦃o,w,v⦄))
+     (wit e)
+     (λ i, ce' i) (ae e)
+     ⦃o,v,sch_c⦄ ⦃o,w⦄
+:=
+begin
+  have
+  : temporal.many_to_many.SPEC₂ v o sch_c ⋀
+      temporal.many_to_many.Wtn ⦃sch_a,w⦄ ⋀
+      ◻(J ! ⦃o,w,v⦄) ⟹
+    temporal.many_to_many.SPEC₁ v o ⋀
+      temporal.many_to_many.SPEC₀.saf w o ⋀
+      ◻(J ! ⦃o,w,v⦄),
+  begin [temporal]
+    simp, intros h₀ h₁ h₂,
+    split*,
+    { apply temporal.many_to_many.SPEC₂_imp_SPEC₁ Hpo ;
+      try { auto }, },
+    { clear Hpo,
+      apply temporal.many_to_many.witness_imp_SPEC₀_saf _ h₀ _ h₁,
+      auto, },
+    { auto }
+  end,
+  constructor ;
+  try { cases (Hpo e w),
+        transitivity, apply this,
+        simp at *,
+        auto, },
+  begin [temporal]
+    intros,
+    casesm* _ ⋀ _,
+    select Hw : temporal.many_to_many.Wtn _,
+    select hJ : ◻(J ! _),
+    have := temporal.many_to_many.H_C_imp_A _ _ _ _ Hw x e
+    ; try { auto <|> apply temporal.many_to_many.sch_w_spec },
+    clear_except this SIM₀ SIM Hw hJ,
+    simp [Wtn] at Hw, cases Hw with Hw Hw,
+    persistent,
+    henceforth at ⊢ this Hw hJ,
+    explicit'
+    { intros, cases Hw,
+      subst w', subst sch_a', subst sch_c,
+      apply this _ _, auto, cc,
+      apply_epsilon_spec, admit,
+      simp, apply SIM ; auto, },
+  end
+end
+
+end Simulation_POs
+
+include H SIM₀ SIM Hpo
+
+lemma sched_ref (i : aevt) -- (w : tvar (aevt × α))
+ (Hw : Γ ⊢ Wtn ⦃sch_a,w⦄)
+ (h : Γ ⊢ ∀∀ j, ref i j ⟶ sched (cs₁ j ! ⦃o,v⦄) (fs₁ j ! ⦃o,v⦄) (sch_c ≃ ↑j ⋀ ⟦ o,v | C j ⟧))
+: Γ ⊢ sched (cs₀ i ! ⦃o,w⦄) (fs₀ i ! ⦃o,w⦄) ⟦ o,w | A i ⟧ :=
+begin [temporal]
+  admit
+  -- have H' := one_to_one.H' C v o sch _ H,
+  -- have hJ : ◻(J ! ⦃o,w,v⦄),
+  -- { replace SIM₀ := SIM₀' _ SIM₀,
+  --   replace SIM := SIM' A C J SIM,
+  --   apply simulation.J_inv_in_w p' q' (Next_a A) _ (J' J) SIM₀ SIM _ o _ H' w Hw },
+  -- simp [J'] at hJ, cases hJ with hJ hJ',
+  -- have Hpo' := Hpo' p q A C cs₁ fs₁ J _ _ _ o sch Hpo (pair.snd ! w) i ; try { auto },
+  -- apply replacement Hpo' Γ _ _,
+  -- clear Hpo Hpo' SIM SIM₀,
+  -- have : ◻ (⦃pair.snd ! w,sch⦄ ≃ w),
+  -- { persistent,
+  --   henceforth at hJ' ⊢,
+  --   explicit
+  --   { clear_except hJ', simp [J'._match_1] at ⊢ hJ',
+  --     rw ← hJ', simp } },
+  -- rw [this], tauto, auto,
+end
+
+lemma many_to_many
+: Γ ⊢ ∃∃ w, SPEC₀ w o :=
+begin [temporal]
+  apply p_exists_partial_intro _ (proj $ @pair.snd aevt α) _ _,
+  select_witness w : temporal.many_to_many.Wtn w with Hw,
+  cases w with sch_a w,
+  have this := H, revert this,
+  dsimp [SPEC₀,SPEC₁],
+  -- have H' := temporal.many_to_many.H' , -- o sch,
+  apply ctx_p_and_p_imp_p_and' _ _,
+  apply ctx_p_and_p_imp_p_and' _ _,
+  { clear_except SIM₀ Hw H,
+    simp [Wtn,SPEC₂] at H Hw,
+    casesm _ ⋀ _,
+    select Hw : (_ ≃ temporal.many_to_many.Wx₀),
+    clear H,
+    explicit'
+    { intro, cases Hw,
+      subst w, apply_epsilon_spec,
+      simp, auto, }, },
+  { clear_except SIM SIM₀ Hw H,
+    have hJ := temporal.many_to_many.J_inv_in_w _ H _ Hw,
+    simp [Wtn,SPEC₂] at H Hw,
+    casesm _ ⋀ _,
+    monotonicity only,
+    simp, intros ce h₀ h₁,
+    select Hw : ◻(_ ≃ _),
+    henceforth at Hw hJ,
+    explicit'
+    { cases Hw, subst w', subst ce,
+      apply_epsilon_spec,
+      simp, auto, }, },
+  { intros h i,
+    apply temporal.many_to_many.sched_ref
+    ; repeat { auto <|> intro }, },
+end
+end SPEC₂
+end conc_sch
+
+section refinement_SPEC₂
+include SIM₀ SIM wit Hpo
+parameters cs₁ fs₁ cs₀ fs₀
+
+-- variable {Γ : cpred}
+
+lemma refinement_SPEC₂
+: Γ ⊢ (∃∃ sch_c, SPEC₂ v o sch_c) ⟶ (∃∃ a, SPEC₀ a o) :=
+begin [temporal]
+  simp, intros sch Hc,
+  apply temporal.many_to_many.many_to_many,
+  auto, auto,
+end
+
+end refinement_SPEC₂
+
+lemma refinement_SPEC₁
+: SPEC₁ v o ⟹ (∃∃ sch, SPEC₂ v o sch) :=
+sorry
+
+end obligations
+
+include SIM₀ SIM
+lemma refinement {o : tvar γ}
+  (h :   ∀ (v : tvar β) (e : aevt) (w : tvar α),
+    many_to_many_po' (subtype (ref e)) (SPEC₁ v o ⋀ SPEC₀.saf w o ⋀ ◻(J ! ⦃o,w,v⦄)) (wit e)
+      (λ (e' : subtype (ref e)), ce ↑e') (ae e)
+      ⦃o,v⦄ ⦃o,w⦄)
+: (∃∃ c, SPEC₁ c o) ⟹ (∃∃ a, SPEC₀ a o) :=
+begin [temporal]
+  transitivity (∃∃ c sch, SPEC₂ q C cs₁ fs₁ c o sch),
+  { apply p_exists_p_imp_p_exists ,
+    intro v,
+    apply refinement_SPEC₁, },
+  { simp, intros c sch Hspec,
+    specialize h c, -- simp [one_to_one_po'] at h,
+    apply temporal.many_to_many.refinement_SPEC₂ c o Γ h,
+    existsi sch, exact Hspec, },
+end
+
+end
+end many_to_many
+
+end temporal
